Cleanup: move lemma around, rename `region.v` -> `memory_region.v`, clean some notations

theories/proofmode/proofmode/memory_region.v
@@ -236,3 +236,23 @@ Section codefrag.
   Qed.
 
 End codefrag.
+
+Section region_addrs_zeroes.
+
+  Definition region_addrs_zeroes (b e : Addr) : list Word :=
+    replicate (finz.dist b e) (WInt 0%Z).
+
+  Lemma region_addrs_zeroes_lookup (b e : Addr) i y :
+    region_addrs_zeroes b e !! i = Some y → y = WInt 0%Z.
+  Proof. apply lookup_replicate. Qed.
+
+  Lemma region_addrs_zeroes_split (b a e: Addr) :
+    (b <= a)%a ∧ (a <= e)%a →
+    region_addrs_zeroes b e = region_addrs_zeroes b a ++ region_addrs_zeroes a e.
+  Proof.
+    intros. rewrite /region_addrs_zeroes.
+    rewrite (finz_dist_split a). 2: solve_addr.
+    rewrite replicate_add //.
+  Qed.
+
+End region_addrs_zeroes.
