theories/case_studies/droe/deep_immutability_spec.v
@@ -16,10 +16,6 @@ Section DROE.
   .
   Context {C : CmptName}.
 
-  Notation STS := (leibnizO (STS_states * STS_rels)).
-  Notation STS_STD := (leibnizO (STS_std_states Addr region_type)).
-  Notation WORLD := (prodO STS_STD STS).
-  Notation CSTK := (leibnizO cstack).
   Implicit Types W : WORLD.
   Implicit Types C : CmptName.
   Notation V := (WORLD -n> (leibnizO CmptName) -n> (leibnizO Word) -n> iPropO Σ).
