theories/logrel/ftlr/WriteSR.v
@@ -19,10 +19,6 @@ Section fundamental.
     {swlayout : switcherLayout}
   .
 
-  Notation STS := (leibnizO (STS_states * STS_rels)).
-  Notation STS_STD := (leibnizO (STS_std_states Addr region_type)).
-  Notation WORLD := (prodO STS_STD STS).
-  Notation CSTK := (leibnizO cstack).
   Implicit Types W : WORLD.
   Implicit Types C : CmptName.
 
@@ -30,7 +26,7 @@ Section fundamental.
   Notation R := (WORLD -n> (leibnizO CmptName) -n> (leibnizO Reg) -n> iPropO Σ).
   Implicit Types w : (leibnizO Word).
   Implicit Types interp : (D).
-  
+
   Lemma writesr_case (W : WORLD) (C : CmptName) (regs : leibnizO Reg)
     (p p' : Perm) (g : Locality) (b e a : Addr)
     (w : Word) (ρ : region_type) (dst : SRegName) (src : RegName) (P:D) (cstk : CSTK) (Ws : list WORLD) (Cs : list CmptName) (wstk : Word)
