theories/logrel/ftlr/interp_weakening.v
@@ -1,7 +1,7 @@
 From iris.proofmode Require Import proofmode.
 From iris.program_logic Require Import weakestpre adequacy lifting.
 From stdpp Require Import base.
-From cap_machine Require Import addr_reg region monotone.
+From cap_machine Require Import addr_reg memory_region monotone.
 From cap_machine Require Export logrel ftlr_base.
 
 Section fundamental.
@@ -16,10 +16,6 @@ Section fundamental.
     {swlayout : switcherLayout}
   .
 
-  Notation STS := (leibnizO (STS_states * STS_rels)).
-  Notation STS_STD := (leibnizO (STS_std_states Addr region_type)).
-  Notation WORLD := (prodO STS_STD STS).
-  Notation CSTK := (leibnizO cstack).
   Implicit Types W : WORLD.
   Implicit Types C : CmptName.
 
