theories/logrel/logrel.v
@@ -1,6 +1,6 @@
 From iris.proofmode Require Import proofmode.
 From iris.program_logic Require Export weakestpre.
-From cap_machine Require Export cap_lang region seal_store region_invariants.
+From cap_machine Require Export cap_lang memory_region seal_store region_invariants.
 From iris.algebra Require Export gmap agree auth excl_auth.
 From iris.base_logic Require Export invariants na_invariants saved_prop.
 From cap_machine Require Import rules_base.
@@ -38,10 +38,8 @@ Record cframe := MkCFrame {
       is_untrusted_caller : bool;
   }.
 
-Notation cstack := (list cframe).
-
-Definition cstackR := excl_authR (leibnizO cstack).
-Definition cstackUR := excl_authUR (leibnizO cstack).
+Definition cstackR := excl_authR (leibnizO (list cframe)).
+Definition cstackUR := excl_authUR (leibnizO (list cframe)).
 
 Class CSTACK_preG Σ :=
   { cstack_preG :: inG Σ cstackUR; }.
@@ -60,6 +58,7 @@ Proof. solve_inG. Qed.
 
 Section CStack.
   Context {Σ : gFunctors} {cstackg : CSTACKG Σ} .
+  Notation cstack := (list cframe).
 
   Definition cstack_full (cstk : cstack) : iProp Σ
     := own γcstack (●E (cstk : leibnizO cstack) : cstackUR).
@@ -97,6 +96,7 @@ End CStack.
 
 Section pre_CSTACK.
   Context {Σ : gFunctors} {tframeg : CSTACK_preG Σ}.
+  Notation cstack := (list cframe).
 
   Lemma gen_cstack_init (cstk : cstack) :
     ⊢ |==> (∃ (cstackg : CSTACKG Σ), cstack_full cstk ∗ cstack_frag cstk).
@@ -122,13 +122,8 @@ Section logrel.
     `{MP: MachineParameters}
     {swlayout : switcherLayout}
   .
-
-  Notation STS := (leibnizO (STS_states * STS_rels)).
-  Notation STS_STD := (leibnizO (STS_std_states Addr region_type)).
-  Notation WORLD := (prodO STS_STD STS).
+  Notation cstack := (list cframe).
   Notation CSTK := (leibnizO cstack).
-  Implicit Types W : WORLD.
-  Implicit Types C : CmptName.
 
   Notation E := (CSTK -n> list WORLD -n> leibnizO (list CmptName) -n> WORLD -n> (leibnizO CmptName) -n> (leibnizO Word) -n> (leibnizO Word) -n> iPropO Σ).
   Notation V := (WORLD -n> (leibnizO CmptName) -n> (leibnizO Word) -n> iPropO Σ).
@@ -136,6 +131,8 @@ Section logrel.
   Notation R := (WORLD -n> (leibnizO CmptName) -n> (leibnizO Reg) -n> iPropO Σ).
   Implicit Types w : (leibnizO Word).
   Implicit Types interp : (V).
+  Implicit Types W : WORLD.
+  Implicit Types C : CmptName.
 
   Definition safeC (P : V) :=
     (λ WCv : WORLD * CmptName * (leibnizO Word), P WCv.1.1 WCv.1.2 WCv.2).
@@ -183,8 +180,6 @@ Section logrel.
   (* interp expression definitions *)
   Definition registers_pointsto (r : Reg) : iProp Σ :=
     ([∗ map] r↦w ∈ r, r ↦ᵣ w)%I.
-
-  Definition SP : RegName := r_t31.
 
   Definition full_map (reg : Reg) : iProp Σ := (∀ (r : RegName), ⌜is_Some (reg !! r)⌝)%I.
   Program Definition interp_reg (interp : V) : R :=
@@ -732,6 +727,7 @@ Section logrel.
 
 
   (* Inversion lemmas about interp  *)
+  (* Inversion lemmas about about when R-capability *)
   Lemma read_allowed_inv (W : WORLD) (C : CmptName) (a' a b e: Addr) p g :
     (b ≤ a' ∧ a' < e)%Z →
     readAllowed p →
@@ -761,6 +757,77 @@ Section logrel.
     iExists p',P'; iFrame "#∗%"; try done.
   Qed.
 
+  Lemma read_allowed_inv_many (W : WORLD) (C : CmptName) (a b e: Addr) p g l :
+    readAllowed p →
+    Forall (fun a' : Addr => (b <= a' < e)%a ) l ->
+    ⊢ (interp W C (WCap p g b e a)) →
+    [∗ list] a' ∈ l,
+          (
+            ∃ (p' : Perm) (P:V),
+              ⌜ PermFlowsTo p p'⌝
+              ∗ ⌜persistent_cond P⌝
+              ∗ rel C a' p' (safeC P)
+              ∗ ▷ zcond P C
+              ∗ ▷ rcond P C p' interp
+              ∗ (if writeAllowed p' then (▷ wcond P C interp) else True)
+              ∗ monoReq W C a' p' P
+          ).
+  Proof.
+    induction l; iIntros (Hra Hin) "#Hinterp"; first done.
+    simpl.
+    apply Forall_cons in Hin. destruct Hin as [Hin_a0 Hin].
+    iDestruct (read_allowed_inv _ _ a0 with "Hinterp")
+      as (p' P) "(%Hperm_flow & %Hpers_P & Hrel_P & Hzcond_P & Hrcond_P & Hwcond_P & HmonoV)"
+    ; auto.
+    iFrame "%#".
+    iApply (IHl with "Hinterp"); eauto.
+  Qed.
+
+  Lemma read_allowed_inv_full_cap (W : WORLD) (C : CmptName) (a b e: Addr) p g :
+    readAllowed p →
+    ⊢ (interp W C (WCap p g b e a)) →
+    [∗ list] a' ∈ (finz.seq_between b e),
+          (
+            ∃ (p' : Perm) (P:V),
+              ⌜ PermFlowsTo p p'⌝
+              ∗ ⌜persistent_cond P⌝
+              ∗ rel C a' p' (safeC P)
+              ∗ ▷ zcond P C
+              ∗ ▷ rcond P C p' interp
+              ∗ (if writeAllowed p' then (▷ wcond P C interp) else True)
+              ∗ monoReq W C a' p' P
+          ).
+  Proof.
+    iIntros (Hra) "Hinterp".
+    iApply (read_allowed_inv_many with "Hinterp"); eauto.
+    apply Forall_forall.
+    intros a' Ha'.
+    by apply elem_of_finz_seq_between.
+  Qed.
+
+  Lemma readAllowed_valid_cap_implies (W : WORLD) (C : CmptName) p g b e a a':
+    readAllowed p = true ->
+    withinBounds b e a' = true ->
+    interp W C (WCap p g b e a) -∗
+    ⌜∃ ρ, std W !! a' = Some ρ ∧ ρ <> Revoked⌝.
+  Proof.
+    intros Hra Hb. iIntros "Hinterp".
+    eapply withinBounds_le_addr in Hb.
+    rewrite /interp. cbn.
+    rewrite fixpoint_interp1_eq interp1_eq; cbn.
+    replace (isO p) with false.
+    2: { eapply readAllowed_nonO in Hra ;done. }
+    destruct (has_sreg_access p) eqn:HnXSR; auto.
+    iDestruct "Hinterp" as "[Hinterp %Hloc]".
+    iDestruct (extract_from_region_inv with "Hinterp")
+             as (p' P' Hfl' Hpers') "(Hrel & Hzcond & Hrcond & Hwcond & HmonoR & %Hstate)";eauto.
+    iPureIntro.
+    destruct (isWL p); simplify_eq.
+    + naive_solver.
+    + destruct g; naive_solver.
+  Qed.
+
+  (* Inversion lemmas about about when W-capability *)
   Lemma write_allowed_inv (W : WORLD) (C : CmptName) (a' a b e: Addr) p g :
     (b ≤ a' ∧ a' < e)%Z →
     writeAllowed p →
@@ -790,26 +857,52 @@ Section logrel.
     iExists p',P'; iFrame "#∗%"; try done.
   Qed.
 
-  Lemma readAllowed_valid_cap_implies (W : WORLD) (C : CmptName) p g b e a a':
-    readAllowed p = true ->
-    withinBounds b e a' = true ->
-    interp W C (WCap p g b e a) -∗
-    ⌜∃ ρ, std W !! a' = Some ρ ∧ ρ <> Revoked⌝.
+  Lemma write_allowed_inv_many (W : WORLD) (C : CmptName) (a b e: Addr) p g l :
+    writeAllowed p →
+    Forall (fun a' : Addr => (b <= a' < e)%a ) l ->
+    ⊢ (interp W C (WCap p g b e a)) →
+    [∗ list] a' ∈ l,
+          (
+            ∃ (p' : Perm) (P:V),
+              ⌜ PermFlowsTo p p'⌝
+              ∗ ⌜persistent_cond P⌝
+              ∗ rel C a' p' (safeC P)
+              ∗ ▷ zcond P C
+              ∗ (if readAllowed p' then (▷ rcond P C p' interp) else True)
+              ∗ (▷ wcond P C interp)
+              ∗ monoReq W C a' p' P
+          ).
   Proof.
-    intros Hra Hb. iIntros "Hinterp".
-    eapply withinBounds_le_addr in Hb.
-    rewrite /interp. cbn.
-    rewrite fixpoint_interp1_eq interp1_eq; cbn.
-    replace (isO p) with false.
-    2: { eapply readAllowed_nonO in Hra ;done. }
-    destruct (has_sreg_access p) eqn:HnXSR; auto.
-    iDestruct "Hinterp" as "[Hinterp %Hloc]".
-    iDestruct (extract_from_region_inv with "Hinterp")
-             as (p' P' Hfl' Hpers') "(Hrel & Hzcond & Hrcond & Hwcond & HmonoR & %Hstate)";eauto.
-    iPureIntro.
-    destruct (isWL p); simplify_eq.
-    + naive_solver.
-    + destruct g; naive_solver.
+    induction l; iIntros (Hra Hin) "#Hinterp"; first done.
+    simpl.
+    apply Forall_cons in Hin. destruct Hin as [Hin_a0 Hin].
+    iDestruct (write_allowed_inv _ _ a0 with "Hinterp")
+      as (p' P) "(%Hperm_flow & %Hpers_P & Hrel_P & Hzcond_P & Hrcond_P & Hwcond_P & HmonoV)"
+    ; auto.
+    iFrame "%#".
+    iApply (IHl with "Hinterp"); eauto.
+  Qed.
+
+  Lemma write_allowed_inv_full_cap (W : WORLD) (C : CmptName) (a b e: Addr) p g :
+    writeAllowed p →
+    ⊢ (interp W C (WCap p g b e a)) →
+    [∗ list] a' ∈ (finz.seq_between b e),
+          (
+            ∃ (p' : Perm) (P:V),
+              ⌜ PermFlowsTo p p'⌝
+              ∗ ⌜persistent_cond P⌝
+              ∗ rel C a' p' (safeC P)
+              ∗ ▷ zcond P C
+              ∗ (if readAllowed p' then (▷ rcond P C p' interp) else True)
+              ∗ (▷ wcond P C interp)
+              ∗ monoReq W C a' p' P
+          ).
+  Proof.
+    iIntros (Hra) "Hinterp".
+    iApply (write_allowed_inv_many with "Hinterp"); eauto.
+    apply Forall_forall.
+    intros a' Ha'.
+    by apply elem_of_finz_seq_between.
   Qed.
 
   Lemma writeAllowed_valid_cap_implies (W : WORLD) (C : CmptName) p g b e a:
@@ -834,19 +927,34 @@ Section logrel.
     + destruct g; naive_solver.
   Qed.
 
-  Lemma writeLocalAllowed_implies_local (W : WORLD) (C : CmptName) p g b e a:
-    isWL p = true ->
-    interp W C (WCap p g b e a) -∗ ⌜ isLocal g = true ⌝.
+  Lemma writeAllowed_valid_cap (W : WORLD) (C : CmptName) p g b e a':
+    writeAllowed p = true ->
+    interp W C (WCap p g b e a') -∗
+    ⌜Forall (fun a => ∃ ρ, std W !! a = Some ρ ∧ ρ <> Revoked) (finz.seq_between b e)⌝.
   Proof.
-    intros. iIntros "Hvalid".
-    unfold interp; rewrite fixpoint_interp1_eq /=.
-    destruct_perm p; simpl in H; try congruence; destruct g; auto.
+    iIntros (Hwa) "Hinterp".
+    rewrite Forall_forall.
+    iIntros (a Ha).
+    apply elem_of_finz_seq_between in Ha.
+    rewrite /interp; cbn.
+    rewrite fixpoint_interp1_eq interp1_eq; cbn.
+    replace (isO p) with false.
+    2: { eapply writeAllowed_nonO in Hwa ;done. }
+    destruct (has_sreg_access p) eqn:HnXSR; auto.
+    iDestruct "Hinterp" as "[Hinterp %Hloc]".
+    iDestruct (extract_from_region_inv with "Hinterp")
+             as (p' P' Hfl' Hpers') "(Hrel & Hzcond & Hrcond & Hwcond & HmonoR & %Hstate)";eauto.
+    iPureIntro.
+    destruct (isWL p); simplify_eq.
+    + naive_solver.
+    + destruct g; naive_solver.
   Qed.
 
-  Lemma writeLocalAllowed_valid_cap_implies (W : WORLD) (C : CmptName) p g b e a:
+  (* Inversion lemmas about about when WL-capability *)
+  Lemma writeLocalAllowed_valid_cap_implies (W : WORLD) (C : CmptName) p g b e a a':
     isWL p = true ->
     withinBounds b e a = true ->
-    interp W C (WCap p g b e a) -∗
+    interp W C (WCap p g b e a') -∗
     ⌜std W !! a = Some Temporary⌝.
   Proof.
     intros Hp Hb. iIntros "Hinterp".
@@ -859,6 +967,40 @@ Section logrel.
     iDestruct (extract_from_region_inv with "Hinterp")
              as (p' P' Hfl' Hpers') "(Hrel & Hzcond & Hrcond & Hwcond & HmonoR & %Hstate)";eauto.
     by rewrite Hp in Hstate.
+  Qed.
+
+  Lemma writeLocalAllowed_valid_cap_implies_many (W : WORLD) (C : CmptName) p g b e a l:
+    isWL p = true ->
+    Forall (fun a' : Addr => (b <= a' < e)%a ) l ->
+    ⊢ (interp W C (WCap p g b e a)) →
+    [∗ list] a' ∈ l, ⌜std W !! a' = Some Temporary⌝.
+  Proof.
+    induction l; iIntros (Hra Hin) "#Hinterp"; first done.
+    simpl.
+    apply Forall_cons in Hin; destruct Hin as [Hin_a0 Hin].
+    iDestruct (writeLocalAllowed_valid_cap_implies with "Hinterp") as "$"; auto.
+    { rewrite /withinBounds; solve_addr. }
+    iApply (IHl with "Hinterp"); eauto.
+  Qed.
+
+  Lemma writeLocalAllowed_valid_cap_implies_full_cap (W : WORLD) (C : CmptName) p g b e a:
+    isWL p = true ->
+    ⊢ (interp W C (WCap p g b e a)) →
+    [∗ list] a' ∈ (finz.seq_between b e), ⌜std W !! a' = Some Temporary⌝.
+  Proof.
+    iIntros (Hwl) "Hinterp".
+    iApply (writeLocalAllowed_valid_cap_implies_many with "Hinterp"); eauto.
+    apply Forall_forall.
+    intros a' Ha'.
+    by apply elem_of_finz_seq_between.
+  Qed.
+
+  Lemma writeLocalAllowed_implies_local (W : WORLD) (C : CmptName) p g b e a:
+    isWL p = true -> interp W C (WCap p g b e a) -∗ ⌜ isLocal g = true ⌝.
+  Proof.
+    intros. iIntros "Hvalid".
+    unfold interp; rewrite fixpoint_interp1_eq /=.
+    destruct_perm p; simpl in H; try congruence; destruct g; auto.
   Qed.
 
   Lemma interp_in_registers
@@ -947,43 +1089,6 @@ Section logrel.
       congruence.
   Qed.
 
-  Lemma writeAllowed_valid_cap (W : WORLD) (C : CmptName) p g b e a':
-    writeAllowed p = true ->
-    interp W C (WCap p g b e a') -∗
-    ⌜Forall (fun a => ∃ ρ, std W !! a = Some ρ ∧ ρ <> Revoked) (finz.seq_between b e)⌝.
-  Proof.
-    iIntros (Hwa) "Hinterp".
-    rewrite Forall_forall.
-    iIntros (a Ha).
-    apply elem_of_finz_seq_between in Ha.
-    rewrite /interp; cbn.
-    rewrite fixpoint_interp1_eq interp1_eq; cbn.
-    replace (isO p) with false.
-    2: { eapply writeAllowed_nonO in Hwa ;done. }
-    destruct (has_sreg_access p) eqn:HnXSR; auto.
-    iDestruct "Hinterp" as "[Hinterp %Hloc]".
-    iDestruct (extract_from_region_inv with "Hinterp")
-             as (p' P' Hfl' Hpers') "(Hrel & Hzcond & Hrcond & Hwcond & HmonoR & %Hstate)";eauto.
-    iPureIntro.
-    destruct (isWL p); simplify_eq.
-    + naive_solver.
-    + destruct g; naive_solver.
-  Qed.
-
-  Lemma is_switcher_entry_point_call :
-    is_switcher_entry_point (WSentry XSRW_ Local b_switcher e_switcher a_switcher_call) = true.
-  Proof.
-    rewrite /is_switcher_entry_point.
-    rewrite bool_decide_eq_true_2; first done.
-    by left.
-  Qed.
-  Lemma is_switcher_entry_point_return :
-    is_switcher_entry_point (WSentry XSRW_ Local b_switcher e_switcher a_switcher_return) = true.
-  Proof.
-    rewrite /is_switcher_entry_point.
-    rewrite bool_decide_eq_true_2; first done.
-    by right.
-  Qed.
   Lemma switcher_call_interp W B :
     ⊢ interp W B (WSentry XSRW_ Local b_switcher e_switcher a_switcher_call).
   Proof.
@@ -998,3 +1103,6 @@ Section logrel.
   Qed.
 
 End logrel.
+
+Notation cstack := (list cframe).
+Notation CSTK := (leibnizO cstack).
