theories/logrel/seal_store.v
@@ -65,9 +65,6 @@ Section Store.
       {Cname : CmptNameG}
       {stsg : STSG Addr region_type Σ}
       {heapg : heapGS Σ}.
-  Notation STS := (leibnizO (STS_states * STS_rels)).
-  Notation STS_STD := (leibnizO (STS_std_states Addr region_type)).
-  Notation WORLD := (prodO STS_STD STS).
   Implicit Types W : WORLD.
 
   Definition seal_pred (o : OType) (P : WORLD * CmptName * Word → iProp Σ) :=
