theories/model/region_invariants.v
@@ -1581,3 +1581,7 @@ Section heap.
   Qed.
 
 End heap.
+
+Notation STS := (leibnizO (STS_states * STS_rels)).
+Notation STS_STD := (leibnizO (STS_std_states Addr region_type)).
+Notation WORLD := (prodO STS_STD STS).
