theories/model/region_invariants_revocation.v
@@ -11,9 +11,6 @@ Section heap.
     {heapg : heapGS Σ}
     `{MP: MachineParameters}.
 
-  Notation STS := (leibnizO (STS_states * STS_rels)).
-  Notation STS_STD := (leibnizO (STS_std_states Addr region_type)).
-  Notation WORLD := (prodO STS_STD STS).
   Implicit Types W : WORLD.
   Implicit Types C : CmptName.
 
